{\bf Problem 1}

\begin{enumerate}[label={\arabic*.}]
    \item $\textrm{MAKES-NOISE}(\textrm{ABIGAIL}) \implies \forall x \, \neg \textrm{CAN-SLEEP}(x)$
    \item $\textrm{MAKES-NOISE}(\textrm{ABIGAIL}) \implies \exists x \, \neg \textrm{CAN-SLEEP}(x)$
    \item $\forall x \textrm{BROTHER} ( \textrm{ABIGAIL}, x ) \implies \neg \textrm{CAN-SLEEP}(x)$
    \item $\exists x \textrm{BROTHER} ( \textrm{ABIGAIL}, x ) \land \textrm{MAKES-NOISE} ( x ) \implies \neg \textrm{CAN-SLEEP} ( \textrm{ABIGAIL} )$
\end{enumerate}
